src/impl/TLS13.Impl.Handle.DecodeError.fst
@@ -1,4 +1,4 @@
-module TLS13.Impl.Handle.Handshake
+module TLS13.Impl.Handle.DecodeError
 
 #lang-pulse
 
@@ -6,17 +6,14 @@ open Pulse.Lib.Pervasives
 open Pulse.Lib.Array.PtsTo
 
 module B = TLS13.Bytes
-module CS = TLS13.Spec.ConnectionState
 module C = TLS13.Impl.ConnectionState
 module CT = TLS13.Impl.Client.Types
-module L = TLS13.Impl.Messages
-module M = TLS13.Messages
+module Seq = FStar.Seq
 module SZ = FStar.SizeT
 module U8 = FStar.UInt8
 
-fn handle_handshake_message
+fn handle_decode_error
   (c:C.connection_state)
-  (l:L.tls_message)
   (raw:array U8.t)
   (raw_len:SZ.t)
   (network_out:array U8.t)
@@ -24,22 +21,43 @@ fn handle_handshake_message
   (app_out:array U8.t)
   (app_out_len:SZ.t)
   requires C.connection_exactly c 'st0 **
-           (exists* m. L.is_valid_tls_message l m) **
            pts_to raw 'raw_bytes **
            pts_to network_out 'old_network_out **
            pts_to app_out 'old_app_out **
            pure (B.length 'raw_bytes == SZ.v raw_len /\
                  B.length 'old_network_out == SZ.v network_out_len /\
-           B.length 'old_app_out == SZ.v app_out_len /\
-           L.tls_message_is_handshake l)
+                 B.length 'old_app_out == SZ.v app_out_len)
   returns resp: CT.client_response
-  ensures exists* st1 m network_out_bytes app_out_bytes.
+  ensures exists* st1 network_out_bytes app_out_bytes.
           C.connection_exactly c st1 **
           pts_to raw 'raw_bytes **
           pts_to network_out network_out_bytes **
           pts_to app_out app_out_bytes **
           pure (B.length network_out_bytes == SZ.v network_out_len /\
                 B.length app_out_bytes == SZ.v app_out_len /\
-                CT.legal_handled_tls_response
-                  'st0 st1 resp m (Ghost.reveal 'raw_bytes) network_out_bytes app_out_bytes /\
-                CT.some_legal_response 'st0 st1 resp network_out_bytes app_out_bytes)
+          CT.decode_error_response 'st0 st1 resp network_out_bytes app_out_bytes /\
+          CT.some_legal_response 'st0 st1 resp network_out_bytes app_out_bytes)
+{
+  C.mark_decode_error c;
+  let resp = {
+    CT.network_out_len = 0sz;
+    CT.app_out_len = 0sz;
+    CT.status = CT.DecodeError;
+  };
+  Seq.lemma_len_slice 'old_network_out 0 0;
+  Seq.lemma_eq_intro B.empty (Seq.slice 'old_network_out 0 0);
+  assert (pure (Seq.equal B.empty (CT.response_network_out resp 'old_network_out)));
+  assert (pure (CT.decode_error_response
+    'st0
+    (C.local_fail_state 'st0 C.tls_decode_error)
+    resp
+    'old_network_out
+    'old_app_out));
+  assert (pure (CT.some_legal_response
+    'st0
+    (C.local_fail_state 'st0 C.tls_decode_error)
+    resp
+    'old_network_out
+    'old_app_out));
+  resp
+}
